src/out/Test.ml
@@ -1,138 +1,217 @@
 open Prims
-let (bc_0x7fec7faa6a80 : Structs.bytecode) =
+let (bc_0x7f1fd820d2f0 : Structs.bytecode) =
   Structs.CODE
     [Structs.LOAD_CONST Prims.int_one;
     Structs.LOAD_CONST (Prims.of_int (2));
     Structs.MAKE_FUNCTION Prims.int_zero;
     Structs.STORE_FAST Prims.int_zero;
-    Structs.LOAD_FAST Prims.int_zero;
-    Structs.CALL_FUNCTION Prims.int_zero;
-    Structs.BUILD_LIST Prims.int_one;
-    Structs.STORE_FAST Prims.int_one;
-    Structs.LOAD_FAST Prims.int_one;
-    Structs.RETURN_VALUE]
-let (bc_0x7fec7faa69d0 : Structs.bytecode) =
-  Structs.CODE
-    [Structs.LOAD_CONST Prims.int_one;
-    Structs.LOAD_CONST (Prims.of_int (2));
     Structs.LOAD_CONST (Prims.of_int (3));
     Structs.LOAD_CONST (Prims.of_int (4));
+    Structs.MAKE_FUNCTION Prims.int_zero;
+    Structs.STORE_FAST Prims.int_one;
+    Structs.LOAD_CLOSURE Prims.int_one;
+    Structs.BUILD_TUPLE Prims.int_one;
     Structs.LOAD_CONST (Prims.of_int (5));
     Structs.LOAD_CONST (Prims.of_int (6));
+    Structs.MAKE_FUNCTION (Prims.of_int (8));
+    Structs.STORE_DEREF Prims.int_one;
     Structs.LOAD_CONST (Prims.of_int (7));
     Structs.LOAD_CONST (Prims.of_int (8));
+    Structs.MAKE_FUNCTION Prims.int_zero;
+    Structs.STORE_DEREF Prims.int_zero;
+    Structs.LOAD_CLOSURE Prims.int_zero;
+    Structs.BUILD_TUPLE Prims.int_one;
     Structs.LOAD_CONST (Prims.of_int (9));
-    Structs.BUILD_LIST (Prims.of_int (9));
-    Structs.STORE_FAST Prims.int_zero;
-    Structs.LOAD_FAST Prims.int_zero;
-    Structs.LOAD_CONST Prims.int_zero;
-    Structs.LOAD_CONST Prims.int_zero;
-    Structs.BUILD_SLICE (Prims.of_int (2));
-    Structs.BINARY_SUBSCR;
-    Structs.STORE_FAST Prims.int_one;
-    Structs.LOAD_FAST Prims.int_zero;
-    Structs.LOAD_CONST Prims.int_zero;
-    Structs.LOAD_CONST Prims.int_zero;
     Structs.LOAD_CONST (Prims.of_int (10));
-    Structs.BUILD_SLICE (Prims.of_int (3));
-    Structs.BINARY_SUBSCR;
+    Structs.MAKE_FUNCTION (Prims.of_int (8));
     Structs.STORE_FAST (Prims.of_int (2));
     Structs.LOAD_FAST Prims.int_zero;
-    Structs.LOAD_CONST Prims.int_zero;
-    Structs.LOAD_CONST Prims.int_zero;
-    Structs.LOAD_CONST (Prims.of_int (2));
-    Structs.BUILD_SLICE (Prims.of_int (3));
-    Structs.BINARY_SUBSCR;
-    Structs.STORE_FAST (Prims.of_int (3));
-    Structs.LOAD_FAST Prims.int_zero;
-    Structs.LOAD_CONST Prims.int_zero;
-    Structs.LOAD_CONST Prims.int_zero;
+    Structs.CALL_FUNCTION Prims.int_zero;
+    Structs.LOAD_FAST Prims.int_one;
     Structs.LOAD_CONST (Prims.of_int (11));
-    Structs.BUILD_SLICE (Prims.of_int (3));
-    Structs.BINARY_SUBSCR;
-    Structs.STORE_FAST (Prims.of_int (4));
-    Structs.LOAD_FAST Prims.int_zero;
     Structs.LOAD_CONST (Prims.of_int (12));
     Structs.LOAD_CONST (Prims.of_int (13));
-    Structs.BUILD_SLICE (Prims.of_int (2));
-    Structs.BINARY_SUBSCR;
-    Structs.STORE_FAST (Prims.of_int (5));
-    Structs.LOAD_FAST Prims.int_zero;
+    Structs.CALL_FUNCTION (Prims.of_int (3));
+    Structs.LOAD_DEREF Prims.int_one;
     Structs.LOAD_CONST (Prims.of_int (14));
-    Structs.LOAD_CONST Prims.int_zero;
-    Structs.LOAD_CONST (Prims.of_int (10));
-    Structs.BUILD_SLICE (Prims.of_int (3));
-    Structs.BINARY_SUBSCR;
-    Structs.STORE_FAST (Prims.of_int (6));
-    Structs.LOAD_FAST Prims.int_zero;
-    Structs.LOAD_CONST (Prims.of_int (5));
+    Structs.CALL_FUNCTION Prims.int_one;
+    Structs.LOAD_FAST (Prims.of_int (2));
+    Structs.CALL_FUNCTION Prims.int_zero;
+    Structs.BUILD_LIST (Prims.of_int (4));
+    Structs.STORE_FAST (Prims.of_int (3));
+    Structs.LOAD_FAST (Prims.of_int (3));
+    Structs.RETURN_VALUE]
+let (bc_0x7f1fd820d240 : Structs.bytecode) =
+  Structs.CODE
+    [Structs.LOAD_DEREF Prims.int_zero;
+    Structs.CALL_FUNCTION Prims.int_zero;
+    Structs.RETURN_VALUE]
+let (consts_0x7f1fd820d240 : Structs.pyObj Prims.list) =
+  [Structs.PYTYP (PyNone.createNone ())]
+let varnames_0x7f1fd820d240 : 'uuuuu . unit -> 'uuuuu Prims.list =
+  fun uu___ -> []
+let names_0x7f1fd820d240 : 'uuuuu . unit -> 'uuuuu Prims.list =
+  fun uu___ -> []
+let cellvars_0x7f1fd820d240 : 'uuuuu . unit -> 'uuuuu Prims.list =
+  fun uu___ -> []
+let (freevars_0x7f1fd820d240 : Prims.string Prims.list) =
+  ["test_function_to_be_called"]
+let (co_0x7f1fd820d240 : Structs.codeObj) =
+  {
+    Structs.co_code = bc_0x7f1fd820d240;
+    Structs.co_consts = consts_0x7f1fd820d240;
+    Structs.co_varnames = (varnames_0x7f1fd820d240 ());
+    Structs.co_names = (names_0x7f1fd820d240 ());
+    Structs.co_cellvars = (cellvars_0x7f1fd820d240 ());
+    Structs.co_freevars = freevars_0x7f1fd820d240
+  }
+let (bc_0x7f1fd820d190 : Structs.bytecode) =
+  Structs.CODE [Structs.LOAD_CONST Prims.int_one; Structs.RETURN_VALUE]
+let (consts_0x7f1fd820d190 : Structs.pyObj Prims.list) =
+  [Structs.PYTYP (PyNone.createNone ());
+  Structs.PYTYP (PyInt.createInt Prims.int_one)]
+let varnames_0x7f1fd820d190 : 'uuuuu . unit -> 'uuuuu Prims.list =
+  fun uu___ -> []
+let names_0x7f1fd820d190 : 'uuuuu . unit -> 'uuuuu Prims.list =
+  fun uu___ -> []
+let cellvars_0x7f1fd820d190 : 'uuuuu . unit -> 'uuuuu Prims.list =
+  fun uu___ -> []
+let freevars_0x7f1fd820d190 : 'uuuuu . unit -> 'uuuuu Prims.list =
+  fun uu___ -> []
+let (co_0x7f1fd820d190 : Structs.codeObj) =
+  {
+    Structs.co_code = bc_0x7f1fd820d190;
+    Structs.co_consts = consts_0x7f1fd820d190;
+    Structs.co_varnames = (varnames_0x7f1fd820d190 ());
+    Structs.co_names = (names_0x7f1fd820d190 ());
+    Structs.co_cellvars = (cellvars_0x7f1fd820d190 ());
+    Structs.co_freevars = (freevars_0x7f1fd820d190 ())
+  }
+let (bc_0x7f1fd820d0e0 : Structs.bytecode) =
+  Structs.CODE
+    [Structs.LOAD_FAST Prims.int_zero;
     Structs.LOAD_CONST Prims.int_one;
-    Structs.BUILD_SLICE (Prims.of_int (2));
-    Structs.BINARY_SUBSCR;
-    Structs.STORE_FAST (Prims.of_int (7));
-    Structs.LOAD_FAST Prims.int_zero;
+    Structs.COMPARE_OP Prims.int_one;
+    Structs.POP_JUMP_IF_FALSE (Prims.of_int (12));
     Structs.LOAD_CONST Prims.int_one;
-    Structs.LOAD_CONST (Prims.of_int (5));
-    Structs.LOAD_CONST (Prims.of_int (10));
-    Structs.BUILD_SLICE (Prims.of_int (3));
-    Structs.BINARY_SUBSCR;
-    Structs.STORE_FAST (Prims.of_int (8));
+    Structs.RETURN_VALUE;
+    Structs.LOAD_FAST Prims.int_zero;
+    Structs.LOAD_DEREF Prims.int_zero;
+    Structs.LOAD_FAST Prims.int_zero;
+    Structs.LOAD_CONST (Prims.of_int (2));
+    Structs.BINARY_SUBTRACT;
+    Structs.CALL_FUNCTION Prims.int_one;
+    Structs.BINARY_ADD;
+    Structs.RETURN_VALUE]
+let (consts_0x7f1fd820d0e0 : Structs.pyObj Prims.list) =
+  [Structs.PYTYP (PyNone.createNone ());
+  Structs.PYTYP (PyInt.createInt Prims.int_zero);
+  Structs.PYTYP (PyInt.createInt Prims.int_one)]
+let (varnames_0x7f1fd820d0e0 : Prims.string Prims.list) = ["x"]
+let names_0x7f1fd820d0e0 : 'uuuuu . unit -> 'uuuuu Prims.list =
+  fun uu___ -> []
+let cellvars_0x7f1fd820d0e0 : 'uuuuu . unit -> 'uuuuu Prims.list =
+  fun uu___ -> []
+let (freevars_0x7f1fd820d0e0 : Prims.string Prims.list) = ["test_recursive"]
+let (co_0x7f1fd820d0e0 : Structs.codeObj) =
+  {
+    Structs.co_code = bc_0x7f1fd820d0e0;
+    Structs.co_consts = consts_0x7f1fd820d0e0;
+    Structs.co_varnames = varnames_0x7f1fd820d0e0;
+    Structs.co_names = (names_0x7f1fd820d0e0 ());
+    Structs.co_cellvars = (cellvars_0x7f1fd820d0e0 ());
+    Structs.co_freevars = freevars_0x7f1fd820d0e0
+  }
+let (bc_0x7f1fd8200f50 : Structs.bytecode) =
+  Structs.CODE
+    [Structs.LOAD_FAST Prims.int_zero;
     Structs.LOAD_FAST Prims.int_one;
     Structs.LOAD_FAST (Prims.of_int (2));
-    Structs.LOAD_FAST (Prims.of_int (3));
-    Structs.LOAD_FAST (Prims.of_int (4));
-    Structs.LOAD_FAST (Prims.of_int (5));
-    Structs.LOAD_FAST (Prims.of_int (6));
-    Structs.LOAD_FAST (Prims.of_int (7));
-    Structs.LOAD_FAST (Prims.of_int (8));
-    Structs.BUILD_TUPLE (Prims.of_int (8));
+    Structs.BUILD_TUPLE (Prims.of_int (3));
     Structs.RETURN_VALUE]
-let (consts_0x7fec7faa69d0 : Structs.pyObj Prims.list) =
+let (consts_0x7f1fd8200f50 : Structs.pyObj Prims.list) =
+  [Structs.PYTYP (PyNone.createNone ())]
+let (varnames_0x7f1fd8200f50 : Prims.string Prims.list) = ["x"; "y"; "z"]
+let names_0x7f1fd8200f50 : 'uuuuu . unit -> 'uuuuu Prims.list =
+  fun uu___ -> []
+let cellvars_0x7f1fd8200f50 : 'uuuuu . unit -> 'uuuuu Prims.list =
+  fun uu___ -> []
+let freevars_0x7f1fd8200f50 : 'uuuuu . unit -> 'uuuuu Prims.list =
+  fun uu___ -> []
+let (co_0x7f1fd8200f50 : Structs.codeObj) =
+  {
+    Structs.co_code = bc_0x7f1fd8200f50;
+    Structs.co_consts = consts_0x7f1fd8200f50;
+    Structs.co_varnames = varnames_0x7f1fd8200f50;
+    Structs.co_names = (names_0x7f1fd8200f50 ());
+    Structs.co_cellvars = (cellvars_0x7f1fd8200f50 ());
+    Structs.co_freevars = (freevars_0x7f1fd8200f50 ())
+  }
+let (bc_0x7f1fd8200df0 : Structs.bytecode) =
+  Structs.CODE [Structs.LOAD_CONST Prims.int_one; Structs.RETURN_VALUE]
+let (consts_0x7f1fd8200df0 : Structs.pyObj Prims.list) =
   [Structs.PYTYP (PyNone.createNone ());
+  Structs.PYTYP (PyInt.createInt Prims.int_one)]
+let varnames_0x7f1fd8200df0 : 'uuuuu . unit -> 'uuuuu Prims.list =
+  fun uu___ -> []
+let names_0x7f1fd8200df0 : 'uuuuu . unit -> 'uuuuu Prims.list =
+  fun uu___ -> []
+let cellvars_0x7f1fd8200df0 : 'uuuuu . unit -> 'uuuuu Prims.list =
+  fun uu___ -> []
+let freevars_0x7f1fd8200df0 : 'uuuuu . unit -> 'uuuuu Prims.list =
+  fun uu___ -> []
+let (co_0x7f1fd8200df0 : Structs.codeObj) =
+  {
+    Structs.co_code = bc_0x7f1fd8200df0;
+    Structs.co_consts = consts_0x7f1fd8200df0;
+    Structs.co_varnames = (varnames_0x7f1fd8200df0 ());
+    Structs.co_names = (names_0x7f1fd8200df0 ());
+    Structs.co_cellvars = (cellvars_0x7f1fd8200df0 ());
+    Structs.co_freevars = (freevars_0x7f1fd8200df0 ())
+  }
+let (consts_0x7f1fd820d2f0 : Structs.pyObj Prims.list) =
+  [Structs.PYTYP
+     (PyString.createString "Tests for calling/defining functions\n    ");
+  Structs.CODEOBJECT co_0x7f1fd8200df0;
+  Structs.PYTYP
+    (PyString.createString
+       "top_level.<locals>.test_function_def_with_no_params");
+  Structs.CODEOBJECT co_0x7f1fd8200f50;
+  Structs.PYTYP
+    (PyString.createString "top_level.<locals>.test_function_def_with_params");
+  Structs.CODEOBJECT co_0x7f1fd820d0e0;
+  Structs.PYTYP (PyString.createString "top_level.<locals>.test_recursive");
+  Structs.CODEOBJECT co_0x7f1fd820d190;
+  Structs.PYTYP
+    (PyString.createString "top_level.<locals>.test_function_to_be_called");
+  Structs.CODEOBJECT co_0x7f1fd820d240;
+  Structs.PYTYP (PyString.createString "top_level.<locals>.test_closure");
   Structs.PYTYP (PyInt.createInt Prims.int_one);
   Structs.PYTYP (PyInt.createInt (Prims.of_int (2)));
   Structs.PYTYP (PyInt.createInt (Prims.of_int (3)));
-  Structs.PYTYP (PyInt.createInt (Prims.of_int (4)));
-  Structs.PYTYP (PyInt.createInt (Prims.of_int (5)));
-  Structs.PYTYP (PyInt.createInt (Prims.of_int (6)));
-  Structs.PYTYP (PyInt.createInt (Prims.of_int (7)));
-  Structs.PYTYP (PyInt.createInt (Prims.of_int (8)));
-  Structs.PYTYP (PyInt.createInt (Prims.of_int (9)));
-  Structs.PYTYP (PyInt.createInt (Prims.of_int (-1)));
-  Structs.PYTYP (PyInt.createInt (Prims.of_int (-2)));
-  Structs.PYTYP (PyInt.createInt Prims.int_zero);
-  Structs.PYTYP (PyInt.createInt (Prims.of_int (15)));
-  Structs.PYTYP (PyInt.createInt (Prims.of_int (-10)))]
-let (varnames_0x7fec7faa69d0 : Prims.string Prims.list) =
-  ["l2"; "x1"; "x2"; "x3"; "x4"; "x5"; "x6"; "x7"; "x8"]
-let names_0x7fec7faa69d0 : 'uuuuu . unit -> 'uuuuu Prims.list =
+  Structs.PYTYP (PyInt.createInt (Prims.of_int (5)))]
+let (varnames_0x7f1fd820d2f0 : Prims.string Prims.list) =
+  ["test_function_def_with_no_params";
+  "test_function_def_with_params";
+  "test_closure";
+  "result"]
+let names_0x7f1fd820d2f0 : 'uuuuu . unit -> 'uuuuu Prims.list =
   fun uu___ -> []
-let (co_0x7fec7faa69d0 : Structs.codeObj) =
-  {
-    Structs.co_code = bc_0x7fec7faa69d0;
-    Structs.co_consts = consts_0x7fec7faa69d0;
-    Structs.co_varnames = varnames_0x7fec7faa69d0;
-    Structs.co_names = (names_0x7fec7faa69d0 ())
-  }
-let (consts_0x7fec7faa6a80 : Structs.pyObj Prims.list) =
-  [Structs.PYTYP
-     (PyString.createString "Test cases for Binary operations\n    ");
-  Structs.CODEOBJECT co_0x7fec7faa69d0;
-  Structs.PYTYP
-    (PyString.createString "top_level.<locals>.test_BINARY_SUBSCR_SLICES")]
-let (varnames_0x7fec7faa6a80 : Prims.string Prims.list) =
-  ["test_BINARY_SUBSCR_SLICES"; "result"]
-let names_0x7fec7faa6a80 : 'uuuuu . unit -> 'uuuuu Prims.list =
+let (cellvars_0x7f1fd820d2f0 : Prims.string Prims.list) =
+  ["test_function_to_be_called"; "test_recursive"]
+let freevars_0x7f1fd820d2f0 : 'uuuuu . unit -> 'uuuuu Prims.list =
   fun uu___ -> []
-let (co_0x7fec7faa6a80 : Structs.codeObj) =
+let (co_0x7f1fd820d2f0 : Structs.codeObj) =
   {
-    Structs.co_code = bc_0x7fec7faa6a80;
-    Structs.co_consts = consts_0x7fec7faa6a80;
-    Structs.co_varnames = varnames_0x7fec7faa6a80;
-    Structs.co_names = (names_0x7fec7faa6a80 ())
+    Structs.co_code = bc_0x7f1fd820d2f0;
+    Structs.co_consts = consts_0x7f1fd820d2f0;
+    Structs.co_varnames = varnames_0x7f1fd820d2f0;
+    Structs.co_names = (names_0x7f1fd820d2f0 ());
+    Structs.co_cellvars = cellvars_0x7f1fd820d2f0;
+    Structs.co_freevars = (freevars_0x7f1fd820d2f0 ())
   }
 let (uu___0 : (Structs.vm * Structs.pyObj)) =
-  VM.runCode_returnVM co_0x7fec7faa6a80
+  VM.runCode_returnVM co_0x7f1fd820d2f0
 let (virt_m : Structs.vm) = match uu___0 with | (virt_m1, res) -> virt_m1
 let (res : Structs.pyObj) = match uu___0 with | (virt_m1, res1) -> res1
 let (print_program_state : unit) =
