src/out/VM.ml
@@ -9,7 +9,9 @@ let (runCode : Structs.codeObj -> Structs.pyObj) =
         Structs.idCount = Prims.int_one;
         Structs.usedIds = Utils.idsMap
       } in
-    let uu___ = Exec.makeFrame initVM code [] Utils.emptyMap Utils.emptyMap in
+    let uu___ =
+      Exec.makeFrame initVM code [] Utils.emptyMap Utils.emptyMap
+        Utils.emptyMap in
     match uu___ with
     | (virM, globalFrame) ->
         let uu___1 = Exec.runFrame virM globalFrame in
@@ -24,7 +26,9 @@ let (runCode_returnVM : Structs.codeObj -> (Structs.vm * Structs.pyObj)) =
         Structs.idCount = Prims.int_one;
         Structs.usedIds = Utils.idsMap
       } in
-    let uu___ = Exec.makeFrame initVM code [] Utils.emptyMap Utils.emptyMap in
+    let uu___ =
+      Exec.makeFrame initVM code [] Utils.emptyMap Utils.emptyMap
+        Utils.emptyMap in
     match uu___ with
     | (virM, globalFrame) ->
         let uu___1 = Exec.runFrame virM globalFrame in
